ccc26x86/Archi.v
@@ -17,30 +17,22 @@
 (** Architecture-dependent parameters for IA32 *)
 
 Require Import ZArith.
-Require Import compcert.flocq.Appli.Fappli_IEEE.
-Require Import compcert.flocq.Appli.Fappli_IEEE_bits.
+Require Import Fappli_IEEE.
+Require Import Fappli_IEEE_bits.
 
 Definition big_endian := false.
 
 Notation align_int64 := 4%Z (only parsing).
 Notation align_float64 := 4%Z (only parsing).
-(*Lenb: Require Import Coq.Init.Peano. does not help.
-So add the definition manually*)
-
-Fixpoint nat_iter (n:nat) {A} (f:A->A) (x:A) : A :=
-  match n with
-    | O => x
-    | S n' =>f (nat_iter n' f x)
-  end.
 
 Program Definition default_pl_64 : bool * nan_pl 53 :=
-  (true, nat_iter 51 xO xH).
+  (true, iter_nat 51 _ xO xH).
 
 Definition choose_binop_pl_64 (s1: bool) (pl1: nan_pl 53) (s2: bool) (pl2: nan_pl 53) :=
   false.                        (**r always choose first NaN *)
 
 Program Definition default_pl_32 : bool * nan_pl 24 :=
-  (true, nat_iter 22 xO xH).
+  (true, iter_nat 22 _ xO xH).
 
 Definition choose_binop_pl_32 (s1: bool) (pl1: nan_pl 24) (s2: bool) (pl2: nan_pl 24) :=
   false.                        (**r always choose first NaN *)
@@ -51,4 +43,3 @@ Global Opaque big_endian
               default_pl_64 choose_binop_pl_64
               default_pl_32 choose_binop_pl_32
               float_of_single_preserves_sNaN.
-
